Add some clocking decision procedures

src/Lustre/LClocking.v
@@ -14,7 +14,7 @@ From Coq Require Import Permutation.
 From Coq Require Import Program.Basics.
 Open Scope program_scope.
 
-(** * Lustre typing *)
+(** * Lustre clocking *)
 
 (**
 
@@ -286,7 +286,6 @@ Module Type LCLOCKING
         (forall x, Ino x (map stream_name anns) -> ~Exists (Is_fresh_in x) es) ->
         DisjointFresh (Eapp f es None anns)
 
-    (* TODO: check *)
     | DFEreset: forall f es e anns,
         DisjointFreshList (e :: es) ->
         Forall DisjointFresh (e :: es) ->
@@ -294,7 +293,6 @@ Module Type LCLOCKING
         Forall Is_AnonStream (map stream_name anns) ->
         (forall x, Ino x (map stream_name anns) -> ~Exists (Is_fresh_in x) (e :: es)) ->
         DisjointFresh (Eapp f es (Some e) anns).
-
 
     Definition WellFormedAnon (e : exp) : Prop :=
       match e with
@@ -491,56 +489,6 @@ Module Type LCLOCKING
     now setoid_rewrite IH.
   Qed.
 
-  (*
-  Lemma indexes_Is_index_in_nclocks:
-    forall i e,
-      In i (indexes (nclockof e)) ->
-      Is_index_in_nclocks i (nclockof e).
-  Proof.
-    intros * Hin. destruct e; simpl in *.
-    - contradiction.
-    - destruct a as (ty, nck). destruct nck; simpl in *.
-      contradiction. destruct c; inversion_clear Hin; subst.
-      now repeat constructor. now inv H.
-    - destruct a as (ty, nck). destruct nck; simpl in *.
-      contradiction. destruct c; inversion_clear Hin; subst.
-      now repeat constructor. now inv H.
-    - destruct a as (ty, nck). destruct nck; simpl in *.
-      contradiction. destruct c; inversion_clear Hin; subst.
-      now repeat constructor. now inv H.
-    - match goal with |- Is_index_in_nclocks _ ?xs =>
-        induction xs as [|nck anns IH] end. now inv Hin.
-      destruct nck; simpl in *.
-      now constructor 2; apply IH.
-      destruct c. 2:now constructor 2; apply IH.
-      inv Hin. now repeat constructor. now constructor 2; apply IH.
-    - match goal with |- Is_index_in_nclocks _ ?xs =>
-        induction xs as [|nck anns IH] end. now inv Hin.
-      destruct nck; simpl in *.
-      now constructor 2; apply IH.
-      destruct c. 2:now constructor 2; apply IH.
-      inv Hin. now repeat constructor. now constructor 2; apply IH.
-    - match goal with |- Is_index_in_nclocks _ ?xs =>
-        induction xs as [|nck anns IH] end. now inv Hin.
-      destruct nck; simpl in *.
-      now constructor 2; apply IH.
-      destruct c. 2:now constructor 2; apply IH.
-      inv Hin. now repeat constructor. now constructor 2; apply IH.
-    - match goal with |- Is_index_in_nclocks _ ?xs =>
-        induction xs as [|nck anns IH] end. now inv Hin.
-      destruct nck; simpl in *.
-      now constructor 2; apply IH.
-      destruct c. 2:now constructor 2; apply IH.
-      inv Hin. now repeat constructor. now constructor 2; apply IH.
-    - match goal with |- Is_index_in_nclocks _ ?xs =>
-        induction xs as [|nck anns IH] end. now inv Hin.
-      destruct nck; simpl in *.
-      now constructor 2; apply IH.
-      destruct c. 2:now constructor 2; apply IH.
-      inv Hin. now repeat constructor. now constructor 2; apply IH.
-  Qed.
-   *)
-
   Instance wc_exp_Proper:
     Proper (@eq global ==> @Permutation.Permutation (ident * clock)
                 ==> @eq exp ==> iff)
@@ -554,21 +502,107 @@ Module Type LCLOCKING
       eauto with lclocking.
   Qed.
 
-  (*
+  Instance wc_exp_pointwise_Proper:
+    Proper (@eq global ==> @Permutation.Permutation (ident * clock)
+                ==> pointwise_relation _ iff)
+           wc_exp.
+  Proof.
+    intros G G' HG env' env Henv e.
+    now rewrite Henv, HG.
+  Qed.
+
+  Instance Is_AnonStream_pointwise_Proper:
+    Proper (@Permutation.Permutation (ident * clock) ==> pointwise_relation _ iff)
+           Is_AnonStream.
+  Proof.
+    intros G' G EG xo.
+    unfold Is_AnonStream; destruct xo; [now rewrite EG|now intuition].
+  Qed.
+
+  Instance Is_AnonStream_Proper:
+    Proper (@Permutation.Permutation (ident * clock) ==> eq ==> iff)
+           Is_AnonStream.
+  Proof.
+    intros G' G EG xo' xo Exo; subst.
+    unfold Is_AnonStream; destruct xo; [now rewrite EG|now intuition].
+  Qed.
+
+  Instance DisjointFresh_pointwise_Proper:
+    Proper (@Permutation.Permutation (ident * clock) ==> pointwise_relation _ iff)
+           DisjointFresh.
+  Proof.
+    intros G' G EG e.
+    Local Hint Extern 4 (Forall _ (_ ++ _)) => apply Forall_app.
+    induction e using exp_ind2; split; inversion 1; subst;
+      repeat match goal with
+             | H:_ <-> _ |- _ => destruct H
+             | H:Forall (fun e => _ e <-> _ e) _ |- _ => apply Forall_iff_insideout in H
+             | H:Forall _ (_ ++ _) |- _ => apply Forall_app in H as (? & ?)
+             | H:Forall _ (_ :: _) |- _ => apply Forall_hd_tl in H as (? & ?)
+             | H:Forall (Is_AnonStream G') _ |- DisjointFresh G _ => rewrite EG in H
+             | H:Forall (Is_AnonStream G) _ |- DisjointFresh G' _ => rewrite <-EG in H
+             end;
+      eauto 8 using DisjointFresh.
+  Qed.
+
+  Instance DisjointFresh_Proper:
+    Proper (@Permutation.Permutation (ident * clock) ==> eq ==> iff)
+           DisjointFresh.
+  Proof.
+    intros G' G EG e' e Ee; subst.
+    induction e using exp_ind2; split; inversion 1; subst;
+      repeat match goal with
+             | H:_ <-> _ |- _ => destruct H
+             | H:Forall (fun e => _ e <-> _ e) _ |- _ => apply Forall_iff_insideout in H
+             | H:Forall _ (_ ++ _) |- _ => apply Forall_app in H as (? & ?)
+             | H:Forall _ (_ :: _) |- _ => apply Forall_hd_tl in H as (? & ?)
+             | H:Forall (Is_AnonStream G') _ |- DisjointFresh G _ => rewrite EG in H
+             | H:Forall (Is_AnonStream G) _ |- DisjointFresh G' _ => rewrite <-EG in H
+             end;
+      eauto 8 using DisjointFresh.
+  Qed.
+
+  Instance WellFormedAnon_Proper:
+    Proper (@Permutation.Permutation (ident * clock) ==> eq ==> iff)
+           WellFormedAnon.
+  Proof.
+    intros G' G EG e' e Ee; subst.
+    unfold WellFormedAnon.
+    destruct e; try rewrite EG; intuition.
+    now destruct o; rewrite EG in *; intuition.
+    now destruct o; rewrite EG; intuition.
+  Qed.
+
+  Instance WellFormedAnon_pointwise_Proper:
+    Proper (@Permutation.Permutation (ident * clock) ==> pointwise_relation _ iff)
+           WellFormedAnon.
+  Proof.
+    intros env' env Henv e. now rewrite Henv.
+  Qed.
+
   Instance wc_equation_Proper:
     Proper (@eq global ==> @Permutation.Permutation (ident * clock)
                 ==> @eq equation ==> iff)
            wc_equation.
   Proof.
-    intros G1 G2 HG env1 env2 Henv eq1 eq2 Heq.
-    rewrite Heq, HG. destruct eq2 as (xs & es).
-    unfold wc_equation.
-    rewrite (wc_patvar_Forall2_perm _ _ _ _ _ _ Henv).
-    split; intro WCeq; destruct WCeq as (WCeq1 & WCeq2 & WCeq3); split; auto;
-      apply Forall_impl_In with (2:=WCeq1); intros;
-        rewrite Henv in *; auto.
+    intros G1 G2 HG env1 env2 Henv eq1 eq2 Heq; subst.
+    destruct eq2 as (xs & es). unfold wc_equation. rewrite Henv.
+    split.
+    - intros (HA & HB & HC & HD).
+      repeat split; auto.
+      now setoid_rewrite Henv in HD.
+    - intros (HA & HB & HC & HD).
+      repeat split; auto.
+      now setoid_rewrite <-Henv in HD.
   Qed.
-   *)
+
+  Instance wc_equation_pointwise_Proper:
+    Proper (@eq global ==> @Permutation.Permutation (ident * clock)
+                ==> pointwise_relation _ iff)
+           wc_equation.
+  Proof.
+    intros G1 G2 HG env1 env2 Henv eq; subst. now rewrite Henv.
+  Qed.
 
   Lemma wc_env_has_Cbase':
     forall vars x xck,
@@ -615,6 +649,1026 @@ Module Type LCLOCKING
     simpl in *. apply in_map_iff. exists nc. destruct nc. simpl in *.
     now inv He.
   Qed.
+
+  (** Validation *)
+
+  Module OpAux := OperatorsAux Op.
+
+  (* TODO: Move elsewhere? *)
+  Local Ltac DestructMatch :=
+    repeat progress
+           match goal with
+           | H:match ?e with _ => _ end = _ |- _ =>
+             let Heq := fresh "Heq" in
+             destruct e eqn:Heq; try discriminate
+           end.
+
+  (* TODO: add to a database *)
+  Hint Extern 2 (In _ (idck _)) => apply In_idck_exists.
+
+  Section ValidateExpression.
+
+    Variable G : global.
+    Variable venv : Env.t (type * clock).
+
+    Open Scope option_monad_scope.
+
+    Function check_var (x : ident) (ck : clock) : bool :=
+      match Env.find x venv with
+      | None => false
+      | Some (_, xc) => ck ==b xc
+      end.
+
+    Definition check_paired_clocks (nc1 nc2 : nclock) (tc : ann) : bool :=
+      match tc with
+      | (t, (c, None)) => (fst nc1 ==b c) && (fst nc2 ==b c)
+      | _ => false
+      end.
+
+    Function check_merge_clocks {A} (x : ident) (ck : clock) (nc1 nc2 : nclock) (ty : A) : bool :=
+      match nc1, nc2 with
+      | (Con ck1 x1 true, _), (Con ck2 x2 false, _) =>
+        (ck1 ==b ck) && (ck2 ==b ck) && (x1 ==b x) && (x2 ==b x)
+      | _, _ => false
+      end.
+
+    Function check_ite_clocks {A} (ck : clock) (nc1 nc2 : nclock) (ty : A) : bool :=
+      (fst nc1 ==b ck) && (fst nc2 ==b ck).
+
+    Definition add_isub
+               (sub : Env.t ident)
+               (nin : (ident * (type * clock)))
+               (nc : nclock) : Env.t ident :=
+      match snd nc, nin with
+      | Some y, (x, (xt, xc)) => Env.add x y sub
+      | None, _ => sub
+      end.
+
+    Definition add_osub
+               (sub : Env.t ident)
+               (nin : (ident * (type * clock)))
+               (tnc : type * nclock) : Env.t ident :=
+      add_isub sub nin (snd tnc).
+
+    Section CheckInst.
+      Variables (bck : clock) (sub : Env.t ident).
+
+      Fixpoint check_inst (ick ck : clock) : bool :=
+        match ick with
+        | Cbase => (ck ==b bck)
+        | Con ick' x xb =>
+          match ck, Env.find x sub with
+          | Con ck' y yb, Some sx =>
+            (yb ==b xb) && (y ==b sx) && (check_inst ick' ck')
+          | _, _ => false
+          end
+        end.
+    End CheckInst.
+
+    Fixpoint find_base_clock (ick ck : clock) : option clock :=
+      match ick with
+      | Cbase => Some ck
+      | Con ick' _ _ =>
+        match ck with
+        | Cbase => None
+        | Con ck' _ _ => find_base_clock ick' ck'
+        end
+      end.
+
+    Definition check_reset (rt : option (option (list nclock))) : bool :=
+      match rt with
+      | None => true
+      | Some (Some [nckr]) => true
+      | _ => false
+      end.
+
+    Lemma nclockof_clockof:
+      forall e xs ys,
+        nclockof e = xs ->
+        ys = map fst xs ->
+        clockof e = ys.
+    Proof.
+      intros e xs ys NC Hys; subst.
+      now rewrite clockof_nclockof.
+    Qed.
+
+    Fixpoint check_exp (e : exp) : option (list nclock) :=
+      match e with
+      | Econst c => Some ([(Cbase, None)])
+
+      | Evar x (xt, nc) =>
+        match nc with
+        | (xc, Some n) => if (check_var x xc) && (x ==b n) then Some [nc] else None
+        | _ => None
+        end
+
+      | Eunop op e (xt, nc) =>
+        match nc with
+        | (xc, None) =>
+          do nce <- assert_singleton (check_exp e);
+          if xc ==b fst nce then Some [nc] else None
+        | _ => None
+        end
+
+      | Ebinop op e1 e2 (xt, nc) =>
+        match nc with
+        | (xc, None) =>
+          do nc1 <- assert_singleton (check_exp e1);
+          do nc2 <- assert_singleton (check_exp e2);
+          if (xc ==b fst nc1) && (xc ==b fst nc2) then Some [nc] else None
+        | _ => None
+        end
+
+      | Efby e0s es anns =>
+        do nc0s <- oconcat (map check_exp e0s);
+        do ncs <- oconcat (map check_exp es);
+        if forall3b check_paired_clocks nc0s ncs anns
+        then Some (map snd anns) else None
+
+      | Ewhen es x b (tys, nc) =>
+        match nc with
+        | (Con xc y yb, None) =>
+          do nces <- oconcat (map check_exp es);
+          if (x ==b y) && (b ==b yb) && (check_var x xc)
+             && (forall2b (fun '(c, _) _ => equiv_decb xc c) nces tys)
+          then Some (map (fun _ => nc) tys) else None
+        | _ => None
+        end
+
+      | Emerge x e1s e2s (tys, (ck, None)) =>
+        do nc1s <- oconcat (map check_exp e1s);
+        do nc2s <- oconcat (map check_exp e2s);
+        let nc' := (ck, None) in
+        if check_var x ck && (forall3b (check_merge_clocks x ck) nc1s nc2s tys)
+        then Some (map (fun _ => nc') tys) else None
+
+      | Eite e e1s e2s (tys, (ck, None)) =>
+        do nc1s <- oconcat (map check_exp e1s);
+        do nc2s <- oconcat (map check_exp e2s);
+        do (ce, _) <- assert_singleton (check_exp e);
+        let nc' := (ck, None) in
+        if (ce ==b ck) && (forall3b (check_ite_clocks ck) nc1s nc2s tys)
+                       && (length tys <>b 0)
+        then Some (map (fun _ => nc') tys) else None
+
+      | Eapp f es ro anns =>
+        do n <- find_node f G;
+        do nces <- oconcat (map check_exp es);
+        do nin0 <- option_map (fun '(_, (_, ck)) => ck) (hd_error n.(n_in));
+        do nces0 <- option_map fst (hd_error nces);
+        do bck <- find_base_clock nin0 nces0;
+        let isub := fold_left2 add_isub n.(n_in) nces (Env.empty ident) in
+        let sub := fold_left2 add_osub n.(n_out) anns isub in
+        if (forall2b (fun '(_, (_, ck)) '(ck', _) => check_inst bck sub ck ck')
+                     n.(n_in) nces)
+           && (forall2b (fun '(_, (_, ck)) '(_, (ck', _)) => check_inst bck sub ck ck')
+                        n.(n_out) anns)
+           && (check_reset (option_map check_exp ro))
+        then Some (map snd anns) else None
+
+      | _ => None end.
+
+    Definition assert_no_intersection (S1 S2 : PS.t) : option PS.t :=
+      if PS.is_empty (PS.inter S1 S2) then Some (PS.union S1 S2) else None.
+
+    Definition check_anon_name (ann : type * nclock) (U : PS.t) : option PS.t :=
+      match snd (snd ann) with
+      | None => Some U
+      | Some x => if PS.mem x U || Env.mem x venv then None else Some (PS.add x U)
+      end.
+
+    Fixpoint check_disjoint_fresh (e : exp) : option PS.t :=
+      match e with
+      | Econst c => Some PS.empty
+      | Evar x _ => Some PS.empty
+      | Eunop op e _ => check_disjoint_fresh e
+      | Ebinop op e1 e2 _ =>
+        do F1 <- check_disjoint_fresh e1;
+        do F2 <- check_disjoint_fresh e2;
+        assert_no_intersection F1 F2
+      | Efby e0s es anns =>
+        do F0s <- omap check_disjoint_fresh e0s;
+        do Fs <- omap check_disjoint_fresh es;
+        let U := ofold_right assert_no_intersection (Some PS.empty) F0s in
+        ofold_right assert_no_intersection U Fs
+      | Ewhen es x b _ =>
+        do Fs <- omap check_disjoint_fresh es;
+        ofold_right assert_no_intersection (Some PS.empty) Fs
+      | Emerge x ets efs _ =>
+        do FTs <- omap check_disjoint_fresh ets;
+        do FFs <- omap check_disjoint_fresh efs;
+        let U := ofold_right assert_no_intersection (Some PS.empty) FTs in
+        ofold_right assert_no_intersection U FFs
+      | Eite e ets efs _ =>
+        do F <- check_disjoint_fresh e;
+        do FTs <- omap check_disjoint_fresh ets;
+        do FFs <- omap check_disjoint_fresh efs;
+        let U := ofold_right assert_no_intersection (Some F) FTs in
+        ofold_right assert_no_intersection U FFs
+
+      | Eapp f es ro anns =>
+        do Fs <- omap check_disjoint_fresh es;
+        let F := match ro with None => Some PS.empty | Some e => check_disjoint_fresh e end in
+        let U := ofold_right assert_no_intersection F Fs in
+        ofold_right check_anon_name U anns
+      end.
+
+    Definition check_wellformedanon (e : exp) : bool :=
+      match e with
+      | Eapp f es ro anns =>
+        match omap check_disjoint_fresh es with
+        | None => false
+        | Some Fs =>
+          let F := match ro with
+                   | None => Some PS.empty
+                   | Some e => check_disjoint_fresh e
+                   end
+          in
+          isSome (ofold_right assert_no_intersection F Fs)
+        end
+      | _ => isSome (check_disjoint_fresh e)
+      end.
+
+    Definition check_wellformedanon_and_exp (e : exp) : option (list nclock) :=
+      if check_wellformedanon e then check_exp e else None.
+
+    Function check_nclock (x : ident) (nck : nclock) : bool :=
+      let '(ck, nm) := nck in
+      check_var x ck && (match nm with
+                         | None => true
+                         | Some n => n ==b x
+                         end).
+
+    Definition check_equation (eq : equation) : bool :=
+      let '(xs, es) := eq in
+      match oconcat (map check_wellformedanon_and_exp es) with
+      | None => false
+      | Some ncks => forall2b check_nclock xs ncks
+      end.
+
+    Lemma assert_no_intersection_correct:
+      forall F S1 S2,
+        assert_no_intersection S1 S2 = Some F ->
+        F = PS.union S1 S2
+        /\ PS.Empty (PS.inter S1 S2).
+    Proof.
+      unfold assert_no_intersection.
+      intros S1 S2 F NI. DestructMatch; inv NI.
+      auto using PSF.is_empty_2.
+    Qed.
+
+    Lemma ofold_right_assert_no_intersection:
+      forall F Fs F',
+        ofold_right assert_no_intersection (Some F) Fs = Some F' ->
+        F' === (PSUnion (F::Fs))
+        /\ DisjointSetList (F::Fs).
+    Proof.
+      induction Fs; simpl.
+      now inversion_clear 1; split; auto using DisjointSetList; reflexivity.
+      intros F' ANI. DestructMatch.
+      specialize (IHFs _ eq_refl) as (? & ?).
+      take (assert_no_intersection _ _ = Some _)
+           and apply assert_no_intersection_correct in it as (? & ?); subst.
+      take (PS.Equal _ _) and rewrite it.
+      rewrite <-perm_swap, (PSUnion_cons _ (F::Fs)).
+      split; [reflexivity|].
+      constructor; auto. rewrite Forall_forall.
+      intros S IS. apply In_PSUnion in IS.
+      rewrite <-it in IS. now rewrite IS.
+    Qed.
+
+    Lemma DisjointFreshList_app:
+      forall es1 es2,
+        DisjointFreshList (es1 ++ es2)
+        <-> (DisjointFreshList es1
+           /\ DisjointFreshList es2
+           /\ Forall (fun e => forall x, Is_fresh_in x e -> ~Exists (Is_fresh_in x) es2) es1).
+    Proof.
+      induction es1 as [|e es1 IH]; intro es2. now intuition constructor.
+      rewrite <-app_comm_cons. split.
+      - inversion 1 as [|?? DFL1 DFL2]; subst.
+        apply IH in DFL1 as (DF1 & DF2 & DFC).
+        setoid_rewrite Exists_app' in DFL2.
+        setoid_rewrite not_or' in DFL2.
+        repeat split; auto using DisjointFreshList; constructor; auto;
+          now intros x FI; apply DFL2 in FI.
+      - intros (DFL1 & DFL2 & DFC).
+        inversion_clear DFL1 as [|?? DFL3 DFL4].
+        apply Forall_hd_tl in DFC as (DFC1 & DFC2).
+        constructor. now apply IH; intuition.
+        intros x Fx. rewrite Exists_app', not_or'. firstorder.
+    Qed.
+
+    Lemma ofold_right_check_anon_name_correct:
+      forall anns F F',
+        ofold_right check_anon_name (Some F) anns = Some F' ->
+        PS.Subset F F'
+        /\ NoDupo (map stream_name anns)
+        /\ Forall (Is_AnonStream (idck (Env.elements venv))) (map stream_name anns)
+        /\ (forall x, Ino x (map stream_name anns) <-> ~PS.In x F /\ PS.In x F').
+    Proof.
+      induction anns as [|ann anns IH]; simpl.
+      now inversion_clear 1;
+        repeat split; eauto using NoDupo_nil, PSP.subset_refl; intuition.
+      intros F F' OFR. DestructMatch.
+      take (ofold_right check_anon_name _ _ = Some _)
+           and apply IH in it as (SS & ND & FA & INO).
+      destruct ann as (ty, (ck, nm)). destruct nm.
+      - unfold check_anon_name in OFR; simpl in *.
+        DestructMatch.
+        take (_ || _ = false) and rewrite Bool.orb_false_iff, <-PSF.not_mem_iff,
+                                         <-Env.Props.P.F.not_mem_in_iff in it.
+        destruct it as (NI & NV). inv OFR. repeat split.
+        + now rewrite SS; apply PSP.subset_add_2.
+        + apply NoDupo_conss; auto.
+          intro Ii; apply INO in Ii as (? & ?); auto.
+        + constructor; auto. simpl.
+          now rewrite InMembers_idck, <-Env.In_Members.
+        + take (_ \/ _) and destruct it; subst; auto.
+          now take (Ino _ _) and apply INO in it as (? & ?).
+        + take (_ \/ _) and destruct it; subst; auto using PSF.add_1.
+          take (Ino _ _) and apply INO in it as (? & ?); auto using PSF.add_2.
+        + intros (Nx & Ix). apply PS.add_spec in Ix as [Ix|Ix]; auto.
+          right. apply INO; auto.
+      - inv OFR; unfold stream_name, Is_AnonStream; simpl.
+        repeat split; auto using NoDupo_consn.
+        + take (_ \/ _) and destruct it; try contradiction;
+            now take (Ino _ _) and apply INO in it as (? & ?).
+        + take (_ \/ _) and destruct it; try contradiction;
+            now take (Ino _ _) and apply INO in it as (? & ?).
+        + intros (Nx & Ix); right. apply INO; auto.
+    Qed.
+
+    Lemma Disjoint_Is_fresh_in_DisjointFreshList:
+      forall es Fs,
+        Forall2 (fun e F => forall x, Is_fresh_in x e <-> PS.In x F) es Fs ->
+        DisjointSetList Fs ->
+        DisjointFreshList es.
+    Proof.
+      induction es as [|e es IH]; auto using DisjointFreshList.
+      intros Fs FA DL. destruct Fs as [|F Fs]; inv FA; inv DL.
+      match goal with DJ:DisjointSetList Fs, FA:Forall2 _ _ _ |- _ =>
+                      specialize (IH _ FA DJ) end.
+      constructor; auto. intros x Fx.
+      take (forall x, Is_fresh_in x _ <-> PS.In x _) and apply it in Fx.
+      apply Forall_Exists_neg.
+      take (Forall2 _ _ _) and apply Forall2_ignore2 in it.
+      apply Forall_impl_In with (2:=it).
+      intros e' Ie' (F' & IF' & HF') Fx'.
+      apply HF' in Fx'.
+      take (Forall _ Fs) and apply Forall_forall with (x:=F') in it; auto.
+      apply PS_disjoint1 with (2:=Fx) in it; auto.
+    Qed.
+
+    Lemma check_disjoint_fresh_correct:
+      forall e F,
+        check_disjoint_fresh e = Some F ->
+        DisjointFresh (idck (Env.elements venv)) e
+        /\ (forall x, Is_fresh_in x e <-> PS.In x F).
+    Proof.
+      assert (forall es1 es2 fs1 fs2,
+                 Forall2 (fun e F => forall x, Is_fresh_in x e <-> PS.In x F) es1 fs1 ->
+                 Forall2 (fun e F => forall x, Is_fresh_in x e <-> PS.In x F) es2 fs2 ->
+                 Forall (fun t => PS.Empty (PS.inter (PSUnion fs1) t)) fs2 ->
+                 Forall (fun e => forall x, Is_fresh_in x e -> ~ Exists (Is_fresh_in x) es2) es1)
+        as L1.
+      { induction es1 as [|e es1 IH]; auto.
+        intros es2 fs1 fs2 FA1 FA2 DJ. inversion FA1 as [|???? FI FA]; subst.
+        constructor.
+        - intros x Fx. apply FI in Fx.
+          apply Forall2_ignore2 in FA2.
+          apply Forall_Exists_neg, Forall_impl_In with (2:=FA2).
+          intros e' Ie' (s & Is & FI') Fx'.
+          apply FI' in Fx'. rewrite Forall_forall in DJ. apply DJ in Is.
+          apply (Is x). rewrite PS.inter_spec, PSUnion_cons.
+          auto using PSF.union_2.
+        - eapply IH; eauto. apply Forall_impl_In with (2:=DJ).
+          intros f If Df x Ix. apply (Df x).
+          apply PS.inter_spec in Ix as (Ix1 & Ix2).
+          apply PS.inter_spec. split; auto.
+          rewrite PSUnion_cons. auto using PSF.union_3. }
+      assert (forall es ss,
+                 Forall2 (fun e s => check_disjoint_fresh e = Some s) es ss ->
+                 Forall (fun e => forall F, check_disjoint_fresh e = Some F ->
+                                    DisjointFresh (idck (Env.elements venv)) e
+                                    /\ (forall x, Is_fresh_in x e <-> PS.In x F)) es ->
+                 Forall (DisjointFresh (idck (Env.elements venv))) es
+                 /\ Forall2 (fun e F => forall x, Is_fresh_in x e <-> PS.In x F) es ss) as L2.
+      { intros es ss FA2 FA. split.
+        - apply Forall2_ignore2 in FA2.
+          apply Forall_impl_In with (2:=FA2).
+          intros e Ie (? & Ix & CDF).
+          rewrite Forall_forall in FA.
+          apply FA with (1:=Ie) in CDF as (? & ?); auto.
+        - apply Forall2_impl_In with (2:=FA2).
+          intros e E Ie IE CDF. rewrite Forall_forall in FA.
+          apply FA with (1:=Ie) in CDF as (? & ?); auto. }
+      assert (forall es ss x t,
+                 Forall2 (fun e F => forall x, Is_fresh_in x e <-> PS.In x F) es ss ->
+                 Forall (fun s => PS.Empty (PS.inter t s)) ss ->
+                 PS.In x t ->
+                 Forall (fun e => ~Is_fresh_in x e) es) as L3.
+      { intros es ss x t FA2 FA Ix.
+        apply Forall2_ignore2 in FA2. apply Forall_impl_In with (2:=FA2).
+        intros e' Ie' (s & Is & Ps) Fs. apply Ps in Fs.
+        apply Forall_forall with (2:=Is) in FA. apply (FA x).
+        auto using PSF.inter_3. }
+      assert (forall es ss x F Fs,
+                 Forall2 (fun e F => forall x : ident, Is_fresh_in x e <-> PS.In x F) es ss ->
+                 Forall (fun s => PS.Empty (PS.inter (PSUnion (F :: Fs)) s)) ss ->
+                 PS.In x F ->
+                 Forall (fun e => ~ Is_fresh_in x e) es) as L4.
+      { intros es ss x F Fx FA2 FA Ix.
+        apply Forall2_ignore2 in FA2. apply Forall_impl_In with (2:=FA2).
+        intros e' Ie' (s & Is & Ps) Fe'. apply Ps in Fe'.
+        apply Forall_forall with (2:=Is) in FA. apply (FA x).
+        rewrite PSUnion_cons. auto using PSF.inter_3, PSF.union_2. }
+      assert (forall x xs ss,
+                 Forall (fun s => PS.Empty (PS.inter (PSUnion (x :: xs)) s)) ss ->
+                 Forall (fun s => PS.Empty (PS.inter (PSUnion xs) s)) ss) as L5.
+      { intros x xs ss FA. apply Forall_impl_In with (2:=FA).
+        intros s Is EI. intro z. specialize (EI z). intro Iz.
+        apply PS.inter_spec in Iz as (? & ?).
+        apply EI, PS.inter_spec. rewrite PSUnion_cons. auto using PSF.union_3. }
+
+      Local Hint Resolve <-Exists_app'.
+      Local Hint Resolve <-Exists_exists.
+      Local Hint Resolve ->Forall_Exists_neg.
+      Local Hint Resolve <-DisjointFreshList_app.
+      Local Hint Constructors DisjointFresh.
+      Local Hint Constructors DisjointFreshList.
+      Local Hint Constructors Is_fresh_in.
+      Local Hint Resolve Disjoint_Is_fresh_in_DisjointFreshList.
+      Local Hint Resolve Forall_app.
+      Local Hint Resolve In_In_PSUnion.
+
+      induction e using exp_ind2; simpl; intros F CD; split;
+        repeat match goal with
+               | ro:option exp |- _ => destruct ro
+               | H:Some _ = Some _ |- _ => inv H
+               | H:_ \/ _ |- _ => destruct H; subst
+               | H:context [ PSUnion (PS.empty :: _) ] |- _ =>
+                 rewrite PSUnion_cons_empty in H
+               | |- context [ PSUnion (_ :: _) ] => rewrite PSUnion_cons
+               | |- context [ PS.In _ (PS.union _ _) ] => rewrite PS.union_spec
+               | |- (forall x, _ <-> _) => intro; split; [inversion_clear 1|intro HH]
+               | H:PS.In ?x PS.empty |- _ => inv H
+               | H:check_disjoint_fresh ?e = Some ?F,
+                 IH:(forall F : PS.t, check_disjoint_fresh ?e = Some F -> _) |- _
+                 => apply IH in H as (? & ?)
+               | H:(forall x, Is_fresh_in x ?e <-> PS.In x ?s) |- _ =>
+                 assert (forall x, Is_fresh_in x e -> PS.In x s) by (setoid_rewrite H; auto);
+                   assert (forall x, PS.In x s -> Is_fresh_in x e) by (setoid_rewrite <-H; auto);
+                   clear H
+               | H:obind ?v _ = Some _ |- _ =>
+                 let OE:=fresh "OE0" in destruct v eqn:OE; [simpl in H|now omonadInv H]
+               | H:forall F, Some _ = Some _ -> _ |- _ => specialize (H _ eq_refl) as (? & ?)
+               | H:assert_no_intersection _ _ = Some _ |- _ =>
+                 apply assert_no_intersection_correct in H as (? & ?); subst
+               | E:PS.Empty (PS.inter _ _) |- _ =>
+                 pose proof (PS_disjoint1 _ _ E); pose proof (PS_disjoint2 _ _ E); clear E
+               | |- PS.In _ (PS.union _ _) => apply PS.union_spec
+               | H:PS.In ?x (PS.union _ _) |- _ => apply PSF.union_1 in H
+               | H: Exists _ (_ ++ _) |- _ => apply Exists_app' in H
+               | H:ofold_right _ (ofold_right assert_no_intersection ?F ?xs) _ = Some F |- _ =>
+                 let OFR:=fresh "OFR" in destruct (ofold_right assert_no_intersection F xs) eqn:OFR
+               | H:ofold_right assert_no_intersection _ _ = Some _ |- _ =>
+                 apply ofold_right_assert_no_intersection in H as (? & ?)
+               | H:ofold_right _ None _ = Some _ |- _ =>
+                 now rewrite ofold_right_none_none in H
+               | H:Forall2 (fun e s => check_disjoint_fresh e = Some s) _ _ |- _ =>
+                 apply L2 in H as (? & ?); [|now auto]
+               | H:Exists (Is_fresh_in _) _ |- _ => apply Exists_exists in H as (? & ? & ?)
+               | H:omap check_disjoint_fresh _ = Some _ |- _ => apply omap_inversion in H
+               | H:ofold_right assert_no_intersection (check_disjoint_fresh ?e) ?xs = Some ?s |- _ =>
+                 let CDF:=fresh "CDF" in destruct (check_disjoint_fresh e) eqn:CDF
+               | H:ofold_right check_anon_name _ _ = Some _ |- _ =>
+                 apply ofold_right_check_anon_name_correct in H as (? & ? & ? & ?)
+               | H:DisjointSetList (_ :: _) |- _ => inv H
+               | T:?t === PSUnion _, H:context [PS.inter ?t _] |- _ =>
+                 setoid_rewrite T in H
+               | EQ:?F === PSUnion ?xs |- PS.In _ ?F => rewrite EQ
+               | EQ:?F === PSUnion ?xs, H:PS.In _ ?F |- _ => rewrite EQ in H
+               | E:?t === PSUnion ?xs |- context [ PS.In _ ?t ] => rewrite E
+               | E:?F === PSUnion (_ :: _), FI:PS.In ?x ?F |- _ => rewrite E in FI
+               | E:?t === PSUnion ?xs, FI:PS.In ?x (PSUnion (?t::?ys)) |- _ =>
+                 let RR:=fresh "RR" in
+                 assert (SetoidList.eqlistA PS.Equal (t :: ys) (PSUnion xs :: ys)) as RR
+                     by (constructor; intuition);
+                   rewrite RR, PSUnion_app, PSUnion_In_app in FI; clear RR
+               | FA:Forall2 (fun e F => forall x, Is_fresh_in x e <-> PS.In x F) ?es ?xs,
+                    Ix:In ?x ?es |- _ =>
+                 apply Forall2_ignore2, Forall_forall with (2:=Ix) in FA as (? & ? & ?)
+               | FA:Forall2 (fun e F => forall x, Is_fresh_in x e <-> PS.In x F) ?es ?Fs,
+                    Ix:In ?x ?Fs |- _ =>
+                 apply Forall2_ignore1, Forall_forall with (2:=Ix) in FA as (? & ? & ?)
+               | H:PS.In ?x (PSUnion ?xs) |- _ =>
+                 apply PSUnion_In_In in H as (? & ? & ?)
+               | H:In ?x (_ :: _) |- _ => apply in_inv in H
+               | H:In _ (_ ++ _) |- _ => apply in_app in H
+               | FP:(forall x, Is_fresh_in x ?e -> PS.In x ?s), FI:Is_fresh_in ?x ?e |- PS.In ?x ?F =>
+                 apply FP in FI
+               | Ix:Ino ?x (map stream_name ?anns),
+                 H:(forall x, Ino x (map stream_name ?anns) <-> _ /\ _) |- _
+                 => apply H in Ix as (? & ?); auto
+               | SS:PS.Subset ?t ?F, TE:?t === PSUnion _ |- PS.In ?x ?F =>
+                 rewrite <-SS, TE, ?PSUnion_cons, ?PS.union_spec; auto
+               end;
+        eauto 20.
+      - (* DisjointFresh (idck (Env.elements venv)) (Ebinop op e1 e2 a) *)
+        constructor; firstorder.
+      - (* DisjointFresh (idck (Env.elements venv)) (Eapp f es (Some e) a) *)
+        constructor; eauto 6.
+        intros x Ix.
+        take (forall x, Ino x (map stream_name _) <-> _ /\ _) and apply it in Ix as (Nx & Ix).
+        take (_ === PSUnion (_ :: _)) and rewrite it, PSUnion_cons, PS.union_spec, not_or' in Nx.
+        destruct Nx as (? & ?).
+        apply Forall_Exists_neg; constructor; auto.
+        take (Forall2 _ _ _) and apply Forall2_ignore2 in it.
+        apply Forall_impl_In with (2:=it).
+        intros e' Ie' (z & Iz & Pz) Fe'.
+        apply Pz in Fe'; eauto.
+      - (* DisjointFresh (idck (Env.elements venv)) (Eapp f es None a) *)
+        constructor; eauto.
+        intros x Ix.
+        take (forall x, Ino x (map stream_name _) <-> _ /\ _) and apply it in Ix as (Nx & Ix).
+        take (_ === PSUnion _) and rewrite it in Nx.
+        apply Forall_Exists_neg.
+        take (Forall2 _ _ _) and apply Forall2_ignore2 in it.
+        apply Forall_impl_In with (2:=it).
+        intros e' Ie' (z & Iz & Pz) Fe'.
+        apply Pz in Fe'; eauto.
+      - (* Is_fresh_in x (Eapp f es (Some e) a) *)
+        constructor.
+        destruct (PSP.In_dec x t) as [Ix|Nx].
+        + left.
+          take (t === PSUnion _) and rewrite it, PSUnion_cons, PS.union_spec in Ix.
+          destruct Ix as [Ix|Ix]; auto.
+          apply PSUnion_In_In in Ix as (? & Ix1 & Ix2).
+          take (Forall2 _ _ _) and apply Forall2_ignore1, Forall_forall
+            with (2:=Ix1) in it as (? & ? & IFI).
+          apply IFI in Ix2; eauto.
+        + right; firstorder.
+      - (* Is_fresh_in x (Eapp f es None a) *)
+        constructor.
+        destruct (PSP.In_dec x t) as [Ix|Nx].
+        + left.
+          take (t === _) and rewrite it in Ix.
+          apply PSUnion_In_In in Ix as (? & Ix1 & Ix2).
+          take (Forall2 _ _ _) and apply Forall2_ignore1 in it;
+            apply Forall_forall with (2:=Ix1) in it as (? & ? & IFI);
+            apply IFI in Ix2; eauto.
+        + right. firstorder.
+    Qed.
+
+    Lemma check_wellformedanon_correct:
+      forall e,
+        check_wellformedanon e = true ->
+        WellFormedAnon (idck (Env.elements venv)) e.
+    Proof.
+      intros e CW.
+      destruct e; simpl in *;
+        try apply isSome_true in CW as (? & ?);
+        eauto using (proj1 (check_disjoint_fresh_correct _ _ _)).
+      DestructMatch.
+      apply isSome_true in CW as (F & CW).
+      match goal with H:omap check_disjoint_fresh ?ls = Some ?ys |- _ =>
+        rename ls into es, ys into Fs, H into CDF end.
+      apply omap_inversion in CDF.
+      assert (Forall (DisjointFresh (idck (Env.elements venv))) es) as DF.
+      { apply Forall2_ignore2 in CDF. apply Forall_impl_In with (2:=CDF).
+        intros e Ie (F' & IF' & CDF').
+        apply check_disjoint_fresh_correct in CDF' as (? & ?); eauto. }
+      assert (Forall2 (fun e F => forall x, Is_fresh_in x e <-> PS.In x F) es Fs) as FI.
+      { apply Forall2_impl_In with (2:=CDF).
+        intros e s Ie Is CDF'.
+        apply check_disjoint_fresh_correct in CDF' as (? & ?); eauto. }
+      take (option exp) and destruct it.
+      - destruct (check_disjoint_fresh e) eqn:CDFe;
+          [|now rewrite ofold_right_none_none in CW].
+        apply ofold_right_assert_no_intersection in CW as (HF & DL).
+        apply check_disjoint_fresh_correct in CDFe as (DFe & FIe).
+        eauto using Disjoint_Is_fresh_in_DisjointFreshList.
+      - apply ofold_right_assert_no_intersection in CW as (HF & DL).
+        inv DL. eauto using Disjoint_Is_fresh_in_DisjointFreshList.
+    Qed.
+
+    Lemma check_var_correct:
+      forall x ck,
+        check_var x ck = true <-> In (x, ck) (idck (Env.elements venv)).
+    Proof.
+      unfold check_var. split; intros HH.
+      - DestructMatch; simpl.
+        rewrite equiv_decb_equiv in HH. inv HH.
+        take (Env.find _ _ = Some _) and apply Env.elements_correct in it; eauto.
+      - apply In_idck_exists in HH as (ty & HH).
+        apply Env.elements_complete in HH as ->.
+        apply equiv_decb_refl.
+    Qed.
+
+    Lemma check_paired_clocks_correct:
+      forall cks1 cks2 anns,
+        forall3b check_paired_clocks cks1 cks2 anns = true ->
+        map stripname cks1 = map clock_of_nclock anns
+        /\ map stripname cks2 = map clock_of_nclock anns
+        /\ Forall unnamed_stream anns.
+    Proof.
+      unfold unnamed_stream.
+      setoid_rewrite forall3b_Forall3.
+      induction 1 as [|(ck1, n1) (ck2, n2) (ty, (ck, n)) cks1 cks2 anns
+                                 IH1 IH2 (Hcks1 & Hcks2 & Hanns)];
+        subst; simpl in *; eauto.
+      destruct n; try discriminate.
+      rewrite Bool.andb_true_iff in IH1.
+      setoid_rewrite equiv_decb_equiv in IH1.
+      destruct IH1 as (Hck1 & Hck2). inv Hck1; inv Hck2.
+      rewrite Hcks1, Hcks2; auto.
+    Qed.
+
+    Lemma check_merge_clocks_correct:
+      forall {A} x ck nc1 nc2 (ty : A),
+        check_merge_clocks x ck nc1 nc2 ty = true ->
+        stripname nc1 = Con ck x true
+        /\ stripname nc2 = Con ck x false.
+    Proof.
+      intros A x ck (ck1, n1) (ck2, n2) ty CM; simpl in CM.
+      DestructMatch; subst.
+      repeat rewrite Bool.andb_true_iff in CM.
+      repeat take (_ /\ _) and destruct it.
+      now repeat take (_ ==b _ = true) and rewrite equiv_decb_equiv in it; inv it.
+    Qed.
+
+    Lemma check_forall3b_merge_clocks_correct:
+      forall {A} x ck ets efs (tys : list A),
+        forall3b (check_merge_clocks x ck) (nclocksof ets) (nclocksof efs) tys = true ->
+        Forall (eq (Con ck x true)) (clocksof ets)
+        /\ Forall (eq (Con ck x false)) (clocksof efs)
+        /\ length (clocksof ets) = length tys
+        /\ length (clocksof efs) = length tys.
+    Proof.
+      setoid_rewrite forall3b_Forall3.
+      intros * FA3. pose proof (Forall3_length _ _ _ _ FA3) as (L1 & L2).
+      setoid_rewrite clocksof_nclocksof; setoid_rewrite Forall_map.
+      setoid_rewrite map_length. rewrite L2, L1, L2.
+      repeat split; auto.
+      - apply Forall3_ignore23 in FA3.
+        apply Forall_impl_In with (2:=FA3).
+        intros nc Inc (y & z & CE).
+        now apply check_merge_clocks_correct in CE as (? & ?).
+      - apply Forall3_ignore13 in FA3.
+        apply Forall_impl_In with (2:=FA3).
+        intros nc Inc (y & z & CE).
+        now apply check_merge_clocks_correct in CE as (? & ?).
+    Qed.
+
+    Lemma check_ite_clocks_correct:
+      forall {A} ck nc1 nc2 (ty : A),
+        check_ite_clocks ck nc1 nc2 ty = true ->
+        stripname nc1 = ck
+        /\ stripname nc2 = ck.
+    Proof.
+      intros A ck (ck1, n1) (ck2, n2) ty CM.
+      unfold check_ite_clocks in CM.
+      rewrite Bool.andb_true_iff in CM.
+      take (_ /\ _) and destruct it.
+      now repeat take (_ ==b _ = true) and rewrite equiv_decb_equiv in it; inv it.
+    Qed.
+
+    Lemma check_forall3b_ite_clocks_correct:
+      forall {A} ck ncs1 ncs2 (tys : list A),
+        forall3b (check_ite_clocks ck) (nclocksof ncs1) (nclocksof ncs2) tys = true ->
+        length (clocksof ncs1) = length tys
+        /\ length (clocksof ncs2) = length tys
+        /\ Forall (eq ck) (clocksof ncs1)
+        /\ Forall (eq ck) (clocksof ncs2).
+    Proof.
+      setoid_rewrite forall3b_Forall3.
+      intros * FA3. pose proof (Forall3_length _ _ _ _ FA3) as (L1 & L2).
+      setoid_rewrite clocksof_nclocksof; setoid_rewrite Forall_map.
+      setoid_rewrite map_length. rewrite L2, L1, L2.
+      repeat split; auto.
+      - apply Forall3_ignore23 in FA3.
+        apply Forall_impl_In with (2:=FA3).
+        intros nc Inc (y & z & CE).
+        now apply check_ite_clocks_correct in CE as (? & ?).
+      - apply Forall3_ignore13 in FA3.
+        apply Forall_impl_In with (2:=FA3).
+        intros nc Inc (y & z & CE).
+        now apply check_ite_clocks_correct in CE as (? & ?).
+    Qed.
+
+    Lemma oconcat_map_check_exp':
+      forall {f} es cks,
+        (forall e cks,
+            In e es ->
+            f e = Some cks ->
+            wc_exp G (idck (Env.elements venv)) e /\ nclockof e = cks) ->
+        oconcat (map f es) = Some cks ->
+        Forall (wc_exp G (idck (Env.elements venv))) es
+        /\ nclocksof es = cks.
+    Proof.
+      induction es as [|e es IH]; intros cks WTf CE. now inv CE; auto.
+      simpl in CE. destruct (f e) eqn:Ce; [|now omonadInv CE].
+      destruct (oconcat (map f es)) as [ces|]; [|now omonadInv CE].
+      omonadInv CE. simpl.
+      apply WTf in Ce as (Ce1 & ->); auto with datatypes.
+      destruct (IH ces) as (? & ->); auto.
+      intros * Ies Fe. apply WTf in Fe; auto with datatypes.
+    Qed.
+
+    Lemma find_add_isub:
+      forall sub x tc ck nm,
+        ~Env.In x sub ->
+        Env.find x (add_isub sub (x, tc) (ck, nm)) = nm.
+    Proof.
+      unfold add_isub; simpl. intros sub x (ty, ck) ? nm NI.
+      destruct nm. now rewrite Env.gss.
+      now apply Env.Props.P.F.not_find_in_iff in NI.
+    Qed.
+
+    Lemma fold_left2_add_osub_skip:
+      forall x xs anns sub,
+        ~In x (map fst xs) ->
+        Env.find x (fold_left2 add_osub xs anns sub) = Env.find x sub.
+    Proof.
+      induction xs as [|(y, (yt, yc)) xs IH]; auto.
+      simpl; intros anns sub NIx.
+      apply Decidable.not_or in NIx as (Nx & NIx).
+      destruct anns as [|(ty, (ck, n)) anns]; auto.
+      rewrite (IH _ _ NIx).
+      unfold add_osub, add_isub; simpl.
+      destruct n; auto.
+      rewrite Env.gso; auto.
+    Qed.
+
+    Lemma fold_left2_add_isub_skip:
+      forall x xs ncs sub,
+        ~In x (map fst xs) ->
+        Env.find x (fold_left2 add_isub xs ncs sub) = Env.find x sub.
+    Proof.
+      induction xs as [|(y, (yt, yc)) xs IH]; auto.
+      simpl; intros ncs sub NIx.
+      apply Decidable.not_or in NIx as (Nx & NIx).
+      destruct ncs as [|(ck, n) anns]; auto.
+      rewrite (IH _ _ NIx).
+      unfold add_isub; simpl.
+      destruct n; auto.
+      rewrite Env.gso; auto.
+    Qed.
+
+    Lemma fold_left2_add_isub:
+      forall x xt xc ck nm xs ncs sub,
+        In ((x, (xt, xc)), (ck, nm)) (combine xs ncs) ->
+        NoDupMembers xs ->
+        ~Env.In x sub ->
+        Env.find x (fold_left2 add_isub xs ncs sub) = nm.
+    Proof.
+      induction xs as [|(y, (yt, yc)) xs IH]. now inversion 1.
+      intros ncs sub Ix ND NI.
+      destruct ncs as [|(ck', nm') ncs]. now inversion Ix.
+      simpl in *.
+      destruct Ix as [Ix|Ix].
+      - inv Ix. inv ND. rewrite fold_left2_add_isub_skip.
+        now apply find_add_isub.
+        rewrite in_map_iff.
+        intros ((y, (yt, yc)) & Fy & Iy). simpl in *; subst.
+        take (~InMembers _ _) and apply it.
+        apply In_InMembers with (1:=Iy).
+      - inv ND. eapply IH in Ix; eauto.
+        apply in_combine_l, In_InMembers in Ix.
+        take (~InMembers _ xs) and apply InMembers_neq with (2:=it) in Ix.
+        unfold add_isub; simpl. destruct nm'; auto.
+        setoid_rewrite Env.Props.P.F.add_in_iff.
+        apply not_or'; auto.
+    Qed.
+
+    Lemma fold_left2_add_osub:
+      forall x xt xc ty ck nm xs ans sub,
+        In ((x, (xt, xc)), (ty, (ck, nm))) (combine xs ans) ->
+        NoDupMembers xs ->
+        ~Env.In x sub ->
+        Env.find x (fold_left2 add_osub xs ans sub) = nm.
+    Proof.
+      induction xs as [|(y, (yt, yc)) xs IH]. now inversion 1.
+      intros ncs sub Ix ND NI.
+      destruct ncs as [|(ck', nm') ncs]. now inversion Ix.
+      simpl in *.
+      destruct Ix as [Ix|Ix].
+      - inv Ix. inv ND. rewrite fold_left2_add_osub_skip.
+        now apply find_add_isub.
+        rewrite in_map_iff.
+        intros ((y, (yt, yc)) & Fy & Iy). simpl in *; subst.
+        take (~InMembers _ _) and apply it.
+        apply In_InMembers with (1:=Iy).
+      - inv ND. eapply IH in Ix; eauto.
+        apply in_combine_l, In_InMembers in Ix.
+        take (~InMembers _ xs) and apply InMembers_neq with (2:=it) in Ix.
+        unfold add_osub, add_isub; simpl. destruct nm'; auto. simpl.
+        destruct o; auto.
+        setoid_rewrite Env.Props.P.F.add_in_iff.
+        apply not_or'; auto.
+    Qed.
+
+    Lemma check_inst_correct:
+      forall bck xc ck sub,
+        check_inst bck sub xc ck = true ->
+        instck bck (fun x => Env.find x sub) xc = Some ck.
+    Proof.
+      induction xc as [|xc' ? x b]; simpl.
+      now setoid_rewrite equiv_decb_equiv; inversion 2.
+      destruct ck. now inversion 1.
+      intros sub Fx. DestructMatch.
+      repeat take (_ && _ = true) and apply andb_prop in it as (? & ?).
+      repeat take ((_ ==b _) = true) and rewrite equiv_decb_equiv in it; inv it.
+      now take (check_inst _ _ _ _ = true) and apply IHxc in it as ->.
+    Qed.
+
+    Lemma check_exp_correct:
+      forall e ncks,
+        check_exp e = Some ncks ->
+        wc_exp G (idck (Env.elements venv)) e
+        /\ nclockof e = ncks.
+    Proof.
+      induction e using exp_ind2; simpl; intros ncks CE;
+      repeat progress
+               match goal with
+               | H:None = Some _ |- _ => discriminate
+               | H:Some _ = Some _ |- _ => inv H
+               | a:ann |- _ => destruct a
+               | a:lann |- _ => destruct a
+               | nc:nclock |- _ => destruct nc
+               | H:obind _ _ = Some _ |- _ => omonadInv H
+               | H: _ && _ = true |- _ => apply Bool.andb_true_iff in H as (? & ?)
+               | H: ((_ ==b _) = true) |- _ => rewrite equiv_decb_equiv in H; inv H
+               | H:(if ?c then Some _ else None) = Some _ |- _ =>
+                 let C := fresh "C0" in
+                 destruct c eqn:C
+               | H:check_var _ _ = true |- _ => apply check_var_correct in H
+               | H:assert_singleton _ = Some _ |- _ => apply assert_singleton_spec in H
+               | H:obind ?v _ = Some _ |- _ =>
+                 let OE:=fresh "OE0" in destruct v eqn:OE; [simpl in H|now omonadInv H]
+               | H:(match ?o with Some _ => _ | None => None end) = Some _ |- _ =>
+                 destruct o
+               | H:(match ?o with Some _ => None | None => _ end) = Some _ |- _ =>
+                 destruct o
+               | H:(match ?c with Cbase => None | _ => _ end) = Some _ |- _ =>
+                 destruct c
+               | H:forall3b check_paired_clocks ?cks1 ?cks2 ?anns = true |- _ =>
+                 apply check_paired_clocks_correct in H as (? & ? & ?)
+               | H:(?xs <>b 0) = true |- _ =>
+                 apply nequiv_decb_true in H;
+                   assert (0 < xs) by (destruct l;
+                     [now exfalso; apply H|apply PeanoNat.Nat.lt_0_succ])
+               | H:obind2 (assert_singleton ?ce) _ = Some _ |- _ =>
+                 destruct (assert_singleton ce) as [(ck, n)|] eqn:AS;
+                   try discriminate; simpl in H
+               end.
+      - (* Econst *)
+        eauto using wc_exp.
+      - (* Evar *)
+        eauto using wc_exp.
+      - (* Eunop *)
+        apply IHe in OE0 as (? & ?).
+        eauto using wc_exp, nclockof_clockof.
+      - (* Ebinop *)
+        apply IHe1 in OE0 as (? & ?); apply IHe2 in OE1 as (? & ?).
+        eauto using wc_exp, nclockof_clockof.
+      - (* Efby *)
+        repeat take (Forall (fun e :exp => _) _) and rewrite Forall_forall in it.
+        apply oconcat_map_check_exp' in OE0 as (? & ?); auto.
+        apply oconcat_map_check_exp' in OE1 as (? & ?); auto. subst.
+        repeat take (map stripname _ = map clock_of_nclock _)
+               and rewrite <-clocksof_nclocksof in it.
+        eauto using wc_exp.
+      - (* Ewhen *)
+        take (Forall _ es) and rewrite Forall_forall in it.
+        take (oconcat (map check_exp _) = Some _) and
+             apply oconcat_map_check_exp' in it as (? & ?); auto.
+        take (forall2b _ _ _ = true) and rename it into FA2; apply forall2b_Forall2 in FA2.
+        subst; simpl; repeat split; auto. constructor; auto; rewrite clocksof_nclocksof.
+        2:rewrite map_length; pose proof (Forall2_length _ _ _ FA2) as Hlen; auto.
+        apply Forall2_ignore2 in FA2. rewrite Forall_map.
+        apply Forall_impl_In with (2:=FA2). intros (? & ?) ? (? & HH).
+        now rewrite equiv_decb_equiv in HH; inv HH.
+      - (* Emerge *)
+        repeat take (Forall _ _) and rewrite Forall_forall in it.
+        repeat take (oconcat (map check_exp _) = Some _) and
+               apply oconcat_map_check_exp' in it as (? & ?); auto.
+        repeat take (nclocksof _ = _) and rewrite <- it in *; clear it.
+        take (forall3b (check_merge_clocks _ _) _ _ _ = true)
+        and apply check_forall3b_merge_clocks_correct in it as (? & ? & ? & ?).
+        eauto using wc_exp.
+      - (* Eite *)
+        repeat take (Forall _ _) and rewrite Forall_forall in it.
+        repeat take (oconcat (map check_exp _) = Some _) and
+               apply oconcat_map_check_exp' in it as (? & ?); auto.
+        repeat take (nclocksof _ = _) and rewrite <- it in *; clear it.
+        take (forall3b (check_ite_clocks _) _ _ _ = true)
+        and apply check_forall3b_ite_clocks_correct in it as (? & ? & ? & ?).
+        apply IHe in AS as (? & ?); auto.
+        eauto using wc_exp, nclockof_clockof.
+      - (* Eapp *)
+        take (Forall _ _) and rewrite Forall_forall in it.
+        take (oconcat (map check_exp _) = Some _) and
+             apply oconcat_map_check_exp' in it as (? & ?); auto.
+        take (nclocksof _ = _) and rewrite <- it in *; clear it.
+        repeat take (forall2b _ _ _ = true) and apply forall2b_Forall2 in it.
+        split; auto.
+        match goal with H:find_base_clock _ _ = Some ?c |- _ => rename c into bck end.
+
+        assert (Forall2 (WellInstantiated bck
+           (fun x => Env.find x (fold_left2 add_osub n.(n_out) a
+              (fold_left2 add_isub n.(n_in) (nclocksof es) (Env.empty _)))))
+                        (idck n.(n_in)) (nclocksof es)).
+        { apply Forall2_map_1, Forall2_forall.
+          take (Forall2 _ n.(n_in) (nclocksof es)) and rename it into FA2.
+          split; [|now apply Forall2_length with (1:=FA2)].
+          intros (x, (xt, xc)) (ck, nm) Ix.
+          constructor; simpl;
+            [|now apply Forall2_In with (1:=Ix), check_inst_correct in FA2].
+          pose proof (NoDupMembers_app_l _ _ n.(n_nodup)).
+          rewrite fold_left2_add_osub_skip, fold_left2_add_isub with (1:=Ix); auto.
+          now rewrite Env.Props.P.F.empty_in_iff.
+          apply in_combine_l, In_InMembers in Ix.
+          rewrite <-fst_InMembers.
+          apply NoDupMembers_app_InMembers with (2:=Ix).
+          pose proof n.(n_nodup) as ND.
+          now rewrite Permutation_swap in ND; apply NoDupMembers_app_r in ND. }
+
+        assert (Forall2 (WellInstantiated bck
+           (fun x => Env.find x (fold_left2 add_osub n.(n_out) a
+             (fold_left2 add_isub n.(n_in) (nclocksof es) (Env.empty ident)))))
+                        (idck n.(n_out)) (map snd a)).
+        { apply Forall2_map_1, Forall2_forall.
+          take (Forall2 _ n.(n_out) _) and rename it into FA2.
+          split; [|now rewrite map_length; apply Forall2_length with (1:=FA2)].
+          intros (x, (xt, xc)) (ck, nm) Ix.
+          rewrite combine_map_snd, in_map_iff in Ix.
+          destruct Ix as (((y & (yt & yc)), (yc' & ynm)) & EE & Ix); inv EE.
+          constructor; simpl.
+          2:now apply Forall2_In with (1:=Ix), check_inst_correct in FA2.
+          pose proof (NoDupMembers_app_r _ _ (NoDupMembers_app_r _ _ n.(n_nodup))).
+          rewrite fold_left2_add_osub with (1:=Ix); auto.
+          setoid_rewrite Env.Props.P.F.not_find_in_iff.
+          rewrite fold_left2_add_isub_skip; auto using Env.gempty.
+          rewrite <-fst_InMembers.
+          apply in_combine_l, In_InMembers in Ix.
+          apply NoDupMembers_app_InMembers with (2:=Ix).
+          rewrite Permutation_app_comm.
+          pose proof n.(n_nodup) as ND.
+          now rewrite Permutation_swap in ND; apply NoDupMembers_app_r in ND. }
+        destruct ro;
+          simpl in *; DestructMatch; subst;
+            try match goal with H:check_exp ?e = Some [?nc] |- _ => destruct nc end;
+            econstructor; eauto;
+            take (forall ncks, Some _ = Some ncks -> _ /\ _) and rename it into CE;
+            specialize (CE _ eq_refl) as (CE1 & CE2); eauto.
+        now apply nclockof_clockof with (1:=CE2).
+    Qed.
+
+    Lemma oconcat_map_check_wellformedanon_and_exp:
+      forall es ncks,
+        oconcat (map check_wellformedanon_and_exp es) = Some ncks ->
+        Forall (wc_exp G (idck (Env.elements venv))) es
+        /\ nclocksof es = ncks
+        /\ Forall (WellFormedAnon (idck (Env.elements venv))) es.
+    Proof.
+      induction es as [|e es IH]; intros ncks CE. now inv CE; eauto.
+      simpl in CE. DestructMatch.
+      take (check_wellformedanon_and_exp _ = Some _) and rename it into CWF.
+      unfold check_wellformedanon_and_exp in CWF.
+      DestructMatch.
+      take (check_wellformedanon _ = true)
+           and apply check_wellformedanon_correct in it.
+      apply check_exp_correct in CWF as (WCe & NCe).
+      destruct (oconcat (map check_wellformedanon_and_exp es)) eqn:CWF; inv CE.
+      specialize (IH _ eq_refl) as (? & ? & ?).
+      simpl. take (nclocksof _ = _) and rewrite it. eauto.
+    Qed.
+
+    Lemma check_equation_correct:
+      forall eq,
+        check_equation eq = true ->
+        wc_equation G (idck (Env.elements venv)) eq.
+    Proof.
+      intros eq CE. destruct eq as (xs, es); simpl in CE.
+      DestructMatch.
+      take (oconcat (map _ _) = Some _)
+      and apply oconcat_map_check_wellformedanon_and_exp in it as (WC & NC & WA).
+      subst. apply forall2b_Forall2 in CE.
+      constructor; auto.
+      rewrite clocksof_nclocksof, Forall2_map_2.
+      split; auto.
+      split; apply Forall2_impl_In with (2:=CE); intros x (ck, nm) Ix Inc CNC;
+        simpl in *; DestructMatch;
+        apply Bool.andb_true_iff in CNC as (CNC1 & CNC2);
+        take (check_var _ _ = true) and apply check_var_correct in it;
+        auto.
+      destruct nm; simpl; auto.
+      now rewrite equiv_decb_equiv in CNC2.
+    Qed.
+
+  End ValidateExpression.
 
 End LCLOCKING.
 
