src/Lustre/LSyntax.v
@@ -219,15 +219,10 @@ Module Type LSYNTAX
         P (Eite e ets efs a).
 
     Hypothesis EappCase:
-      forall f es a,
+      forall f es ro a,
+        (match ro with None => True | Some r => P r end) ->
         Forall P es ->
-        P (Eapp f es None a).
-
-    Hypothesis EresetCase:
-      forall f es r a,
-        P r ->
-        Forall P es ->
-        P (Eapp f es (Some r) a).
+        P (Eapp f es ro a).
 
     Local Ltac SolveForall :=
       match goal with
@@ -246,9 +241,7 @@ Module Type LSYNTAX
       - apply EwhenCase; SolveForall.
       - apply EmergeCase; SolveForall.
       - apply EiteCase; SolveForall; auto.
-      - destruct o.
-        apply EresetCase; SolveForall; auto.
-        apply EappCase; SolveForall.
+      - destruct o; apply EappCase; SolveForall; auto.
     Qed.
 
   End exp_ind2.
